compiler/backend/passes/proofs/pure_to_thunkProofScript.sml
@@ -9,12 +9,13 @@ open stringTheory optionTheory sumTheory pairTheory listTheory alistTheory
      thunkLang_primitivesTheory pure_exp_lemmasTheory pure_miscTheory
      pure_to_thunk_1ProofTheory pure_cexpTheory pureLangTheory
      thunk_case_liftProofTheory
-     thunk_case_d2bProofTheory;
+     thunk_case_d2bProofTheory
+     expof_caseProofTheory;
 
 val _ = new_theory "pure_to_thunkProof";
 
 val _ = set_grammar_ancestry ["pure_to_thunk_1Proof", "pure_cexp",
-                              "thunkLang", "pureLang"];
+                              "thunkLang", "pureLang", "expof_caseProof"];
 
 (*
   cexp = Var 'a vname                         (* variable                 *)
@@ -39,26 +40,26 @@ Definition Apps_def:
 End
 
 Definition lets_for_def:
-  lets_for cn v [] b = b ∧
-  lets_for cn v ((n,w)::ws) b =
-    Let (SOME w) (Delay $ Force $ Prim (Proj cn n) [Force $ Var v]) $
-      lets_for cn v ws b
+  lets_for l cn v [] b = b ∧
+  lets_for l cn v ((n,w)::ws) b =
+    Let NONE (If (Prim (IsEq cn l T) [Force (Var v)]) Unit Fail) $
+      Let (SOME w) (Delay $ Force $ Prim (Proj cn n) [Force $ Var v]) $
+        lets_for l cn v ws b
 End
 
 Definition rows_of_def:
   (rows_of v k [] =
     case k of
-      NONE => Prim (AtomOp Add) []
+      NONE => Fail
     | SOME e => e) ∧
   rows_of v k ((cn,vs,b)::rest) =
    If (Prim (IsEq cn (LENGTH vs) T) [Force (Var v)])
-      (lets_for cn v (MAPi (λi v. (i,v)) vs) b)
+      (lets_for (LENGTH vs) cn v (MAPi (λi v. (i,v)) vs) b)
       (rows_of v k rest)
 End
 
 (*
        | Prim 'a cop (cexp list)                 (* primitive operations     *)
-       | Letrec 'a ((cvname # cexp) list) cexp   (* mutually recursive exps  *)
 *)
 
 Inductive exp_rel:
@@ -85,16 +86,18 @@ Inductive exp_rel:
      LIST_REL exp_rel xs ys ⇒
        exp_rel (App i f xs) (Apps g (MAP Delay ys))) ∧
 [~Case:]
-  (∀i x v xs ys.
+  (∀i x v xs ys fresh.
      ~MEM v (FLAT (MAP (FST ∘ SND) xs)) ∧ xs ≠ [] ∧
-     MAP (explode o FST) xs = MAP FST ys ∧
-     MAP (MAP explode o FST o SND) xs = MAP (FST o SND) ys ∧
-     LIST_REL exp_rel (MAP (SND o SND) xs) (MAP (SND o SND) ys) ∧
+     LIST_REL (λ(x1,x2,x3) (y1,y2,y3).
+       explode x1 = y1 ∧ MAP explode x2 = y2 ∧
+       exp_rel x3 y3 ∧ fresh ∉ freevars (exp_of' x3)) xs ys ∧
+     (∀x. eopt = SOME x ⇒ fresh ∉ freevars (exp_of' x)) ∧
+     exp_rel x a_exp ∧ fresh ≠ explode v ∧
      OPTREL exp_rel eopt yopt ⇒
        exp_rel (Case i x v xs eopt)
          (Let (SOME fresh) a_exp $
           Let (SOME (explode v)) (Box (Var fresh)) $
-            rows_of fresh yopt ys))
+            rows_of (explode v) yopt ys))
 End
 
 Overload to_thunk = “pure_to_thunk_1Proof$compile_rel”
@@ -105,7 +108,9 @@ Theorem LIST_REL_combined_IMP:
   ∀xs ys.
     LIST_REL (λx y.
       exp_rel x y ∧
-      ∃y1 y2. to_thunk (exp_of x) y1 ∧ lift_rel y1 y2 ∧ d2b_rel y2 y) xs ys ⇒
+      (cexp_wf x ⇒
+       ∃y1 y2. to_thunk (exp_of x) y1 ∧ lift_rel y1 y2 ∧ d2b_rel y2 y)) xs ys ∧
+    EVERY (λa. cexp_wf a) xs ⇒
     ∃ts1 ts2.
       LIST_REL (λx y. to_thunk (exp_of x) y) xs ts1 ∧
       LIST_REL lift_rel ts1 ts2 ∧
@@ -148,16 +153,143 @@ Proof
   \\ irule_at Any thunk_case_d2bProofTheory.exp_rel_Delay \\ fs []
 QED
 
+Theorem to_thunk_lets_for:
+  ∀ws. to_thunk rhs rhs' ⇒
+       to_thunk (lets_for' n r0 v ws rhs)
+                (lets_for n r0 v ws rhs')
+Proof
+  Induct \\ fs [lets_for_def,lets_for'_def]
+  \\ PairCases \\ fs [lets_for_def,lets_for'_def] \\ rw [] \\ fs []
+  \\ rpt $ simp [Once pure_to_thunk_1ProofTheory.compile_rel_cases]
+QED
+
+Theorem d2b_lets_for:
+  ∀ws. d2b_rel rhs rhs' ⇒
+       d2b_rel (lets_for n r0 v ws rhs)
+               (lets_for n r0 v ws rhs')
+Proof
+  Induct \\ fs [lets_for_def,lets_for'_def]
+  \\ PairCases \\ fs [lets_for_def,lets_for'_def] \\ rw [] \\ fs []
+  \\ rpt $ simp [Once thunk_case_d2bProofTheory.exp_rel_cases]
+QED
+
+Theorem lift_lets_for:
+  ∀ws. lift_rel rhs rhs' ⇒
+       lift_rel (lets_for n r0 v ws rhs)
+                (lets_for n r0 v ws rhs')
+Proof
+  Induct \\ fs [lets_for_def,lets_for'_def]
+  \\ PairCases \\ fs [lets_for_def,lets_for'_def] \\ rw [] \\ fs []
+  \\ rpt $ simp [Once thunk_case_liftProofTheory.compile_rel_cases]
+QED
+
+Triviality not_freevars_lets_for:
+  fresh ∉ freevars rhs ∧ fresh ≠ y ⇒
+  fresh ∉ freevars (lets_for n x y ws rhs)
+Proof
+  Induct_on ‘ws’ \\ fs [lets_for_def,FORALL_PROD]
+  \\ fs [thunkLangTheory.freevars_def]
+QED
+
+Triviality not_treevars_rows_of:
+  fresh ≠ v ∧
+  EVERY (λ(n,vs,b). fresh ∉ freevars b) rows ∧
+  (∀x. opt = SOME x ⇒ fresh ∉ freevars x) ⇒
+  fresh ∉ freevars (rows_of v opt rows)
+Proof
+  Induct_on ‘rows’ \\ fs [rows_of_def,FORALL_PROD]
+  >- (CASE_TAC \\ fs [freevars_def])
+  \\ rw [freevars_def]
+  \\ irule not_freevars_lets_for \\ fs []
+QED
+
+Theorem d2b_rows_of:
+  ∀rows rows1.
+    LIST_REL (λ(x1,x2,x3) (y1,y2,y3). x1 = y1 ∧ x2 = y2 ∧ d2b_rel x3 y3)
+       rows rows1 ∧ OPTREL d2b_rel opt opt1 ⇒
+    d2b_rel (rows_of v opt rows) (rows_of v opt1 rows1)
+Proof
+  Induct \\ fs [rows_of_def]
+  >-
+   (Cases_on ‘opt’ \\ Cases_on ‘opt1’ \\ fs []
+    \\ rpt $ simp [Once thunk_case_d2bProofTheory.exp_rel_cases])
+  \\ fs [PULL_EXISTS]
+  \\ PairCases
+  \\ PairCases
+  \\ fs [] \\ rw []
+  \\ fs [rows_of_def]
+  \\ simp [Once thunk_case_d2bProofTheory.exp_rel_cases]
+  \\ irule_at Any d2b_lets_for \\ fs []
+  \\ rpt $ simp [Once thunk_case_d2bProofTheory.exp_rel_cases]
+QED
+
+Theorem lift_rows_of:
+  ∀rows rows1.
+    LIST_REL (λ(x1,x2,x3) (y1,y2,y3). x1 = y1 ∧ x2 = y2 ∧ lift_rel x3 y3)
+       rows rows1 ∧ OPTREL lift_rel opt opt1 ⇒
+    lift_rel (rows_of v opt rows) (rows_of v opt1 rows1)
+Proof
+  Induct \\ fs [rows_of_def]
+  >-
+   (Cases_on ‘opt’ \\ Cases_on ‘opt1’ \\ fs []
+    \\ rpt $ simp [Once thunk_case_liftProofTheory.compile_rel_cases])
+  \\ fs [PULL_EXISTS]
+  \\ PairCases
+  \\ PairCases
+  \\ fs [] \\ rw []
+  \\ fs [rows_of_def]
+  \\ simp [Once thunk_case_liftProofTheory.compile_rel_cases]
+  \\ irule_at Any lift_lets_for \\ fs []
+  \\ rpt $ simp [Once thunk_case_liftProofTheory.compile_rel_cases]
+QED
+
+Theorem OPTREL_SIMP:
+  (OPTREL P (SOME x) m ⇔ ∃y. m = SOME y ∧ P x y) ∧
+  (OPTREL P n (SOME y) ⇔ ∃x. n = SOME x ∧ P x y) ∧
+  (OPTREL P NONE m ⇔ m = NONE) ∧
+  (OPTREL P n NONE ⇔ n = NONE)
+Proof
+  Cases_on ‘n’ \\ Cases_on ‘m’ \\ fs []
+QED
+
+Theorem to_thunk_rows_of:
+  ∀xs ys.
+    LIST_REL (λ(x1,x2,x3) (y1,y2,y3).
+        explode x1 = y1 ∧ MAP explode x2 = y2 ∧
+        to_thunk (exp_of' x3) y3)
+      xs ys ∧
+    OPTREL (λe1 e2. to_thunk (exp_of' e1) e2) eopt opt ⇒
+    to_thunk (rows_of' v
+               (case eopt of NONE => Fail | SOME e => exp_of' e)
+               (MAP (λ(c,vs,x'). (explode c,MAP explode vs,exp_of' x')) xs))
+             (rows_of v opt ys)
+Proof
+  Induct \\ fs [PULL_EXISTS]
+  >-
+   (rw [rows_of'_def,rows_of_def]
+    \\ CASE_TAC \\ gvs [OPTREL_SIMP]
+    \\ simp [Once pure_to_thunk_1ProofTheory.compile_rel_cases])
+  \\ fs [UNCURRY] \\ rw [] \\ res_tac
+  \\ rename [‘explode (FST xx) = FST yy’]
+  \\ PairCases_on ‘xx’ \\ PairCases_on ‘yy’ \\ gvs []
+  \\ rw [rows_of'_def,rows_of_def]
+  \\ simp [Once pure_to_thunk_1ProofTheory.compile_rel_cases]
+  \\ simp [Once pure_to_thunk_1ProofTheory.compile_rel_cases]
+  \\ simp [Once pure_to_thunk_1ProofTheory.compile_rel_cases]
+  \\ irule to_thunk_lets_for \\ fs []
+QED
+
+val to_thunk_freevars = pure_to_thunk_1ProofTheory.compile_rel_freevars;
+
 Theorem exp_rel_imp_combined:
   ∀x y.
-    exp_rel x y ⇒
+    exp_rel x y ∧ cexp_wf x ⇒
     ∃y1 y2.
-      to_thunk (exp_of x) y1 ∧
+      to_thunk (exp_of' x) y1 ∧
       lift_rel y1 y2 ∧
       d2b_rel y2 y
 Proof
-
-  Induct_on ‘exp_rel’ \\ rw [pureLangTheory.exp_of_def]
+  Induct_on ‘exp_rel’ \\ rw [exp_of'_def,cexp_wf_def] \\ fs []
   >~ [‘Var n’] >-
    (simp [Once pure_to_thunk_1ProofTheory.compile_rel_cases]
     \\ irule_at Any thunk_case_liftProofTheory.compile_rel_Force
@@ -175,7 +307,7 @@ Proof
     \\ first_x_assum $ irule_at Any
     \\ simp [Once pure_to_thunk_1ProofTheory.compile_rel_cases])
   >~ [‘Let’] >-
-   (irule_at Any pure_to_thunk_1ProofTheory.compile_rel__Let
+   (irule_at Any pure_to_thunk_1ProofTheory.compile_rel_Let
     \\ first_x_assum $ irule_at $ Pos hd
     \\ first_x_assum $ irule_at $ Pos hd
     \\ irule_at Any thunk_case_liftProofTheory.compile_rel_Let
@@ -187,10 +319,11 @@ Proof
   >~ [‘Letrec’] >-
    (irule_at Any thunk_case_d2bProofTheory.exp_rel_Letrec
     \\ irule_at Any thunk_case_liftProofTheory.compile_rel_Letrec
-    \\ irule_at Any pure_to_thunk_1ProofTheory.compile_rel__Letrec
+    \\ irule_at Any pure_to_thunk_1ProofTheory.compile_rel_Letrec
     \\ rpt $ first_assum $ irule_at Any
     \\ last_x_assum mp_tac
     \\ rename [‘LIST_REL _ xs ys’]
+    \\ qpat_x_assum ‘EVERY _ _’ mp_tac
     \\ qid_spec_tac ‘ys’
     \\ qid_spec_tac ‘xs’
     \\ Induct \\ fs [PULL_EXISTS,EXISTS_PROD,FORALL_PROD]
@@ -199,16 +332,80 @@ Proof
     \\ irule_at Any thunk_case_liftProofTheory.compile_rel_Delay
     \\ rpt $ first_assum $ irule_at Any)
   >~ [‘Apps’] >-
-   (drule LIST_REL_combined_IMP \\ strip_tac
-    \\ qexists_tac ‘Apps y1 (MAP Delay ts1)’
-    \\ qexists_tac ‘Apps y2 (MAP Delay ts2)’
+   (irule_at Any lift_rel_Apps \\ fs []
+    \\ irule_at Any d2b_rel_Apps \\ fs []
     \\ irule_at Any to_thunk_Apps \\ simp [listTheory.LIST_REL_MAP1]
-    \\ fs [combinTheory.o_DEF,SF ETA_ss]
-    \\ irule_at Any lift_rel_Apps \\ fs []
-    \\ irule_at Any d2b_rel_Apps \\ fs [])
+    \\ rpt $ first_assum $ irule_at Any
+    \\ qpat_x_assum ‘LIST_REL _ xs ys’ mp_tac
+    \\ qpat_x_assum ‘EVERY _ _’ mp_tac
+    \\ qid_spec_tac ‘ys’
+    \\ qid_spec_tac ‘xs’
+    \\ Induct \\ fs [PULL_EXISTS,EXISTS_PROD,FORALL_PROD]
+    \\ rw [] \\ gvs []
+    \\ res_tac
+    \\ rpt $ first_assum $ irule_at Any)
   >~ [‘rows_of’] (* i.e. Case *)
-
-  \\ cheat
+  \\ Cases_on ‘xs’ >- fs [] \\ gvs []
+  \\ rename [‘MEM v (FST (SND r))’] \\ PairCases_on ‘r’ \\ gvs []
+  \\ rename [‘LIST_REL _ xs ys’]
+  \\ gvs [UNCURRY]
+  \\ rename [‘exp_rel r2 (SND (SND q))’] \\ PairCases_on ‘q’ \\ gvs []
+  \\ irule_at Any pure_to_thunk_1ProofTheory.compile_rel_Let
+  \\ gvs [rows_of'_def]
+  \\ irule_at Any pure_to_thunk_1ProofTheory.compile_rel_If \\ fs []
+  \\ irule_at Any pure_to_thunk_1ProofTheory.compile_rel_Prim \\ fs [PULL_EXISTS]
+  \\ irule_at Any pure_to_thunk_1ProofTheory.compile_rel_Var \\ fs []
+  \\ qpat_x_assum ‘to_thunk (exp_of' x) _’ $ irule_at Any
+  \\ irule_at Any thunk_case_liftProofTheory.compile_rel_Let
+  \\ irule_at Any thunk_case_liftProofTheory.compile_rel_Delay
+  \\ qpat_x_assum ‘lift_rel y1 y2’ $ irule_at Any
+  \\ irule_at (Pos $ hd) thunk_case_liftProofTheory.compile_rel_Lift
+  \\ gvs [thunkLangTheory.freevars_def]
+  \\ irule_at (Pos $ last) thunk_case_d2bProofTheory.exp_rel_D2B \\ fs [rows_of_def]
+  \\ irule_at Any thunk_case_liftProofTheory.compile_rel_Force
+  \\ irule_at Any thunk_case_liftProofTheory.compile_rel_Var
+  \\ irule_at (Pos $ hd) thunk_case_d2bProofTheory.exp_rel_If \\ fs []
+  \\ irule_at (Pos $ hd) thunk_case_d2bProofTheory.exp_rel_Prim \\ fs []
+  \\ irule_at (Pos $ hd) thunk_case_d2bProofTheory.exp_rel_Force \\ fs []
+  \\ irule_at (Pos $ hd) thunk_case_d2bProofTheory.exp_rel_Var \\ fs []
+  \\ irule_at Any to_thunk_lets_for
+  \\ first_assum $ irule_at $ Pos hd
+  \\ irule_at Any d2b_lets_for
+  \\ irule_at Any lift_lets_for
+  \\ first_assum $ irule_at $ Pos hd
+  \\ first_assum $ irule_at $ Pos hd
+  \\ irule_at Any not_freevars_lets_for
+  \\ irule_at Any d2b_rows_of \\ fs []
+  \\ irule_at Any lift_rows_of \\ fs []
+  \\ irule_at Any not_treevars_rows_of \\ fs []
+  \\ irule_at Any to_thunk_rows_of
+  \\ ‘∃ys1 ys2.
+         EVERY (λ(n,vs,b). fresh ∉ freevars b) ys1 ∧
+         LIST_REL
+            (λ(x1,x2,x3) (y1,y2,y3).
+                 explode x1 = y1 ∧ MAP explode x2 = y2 ∧
+                 to_thunk (exp_of' x3) y3) xs ys1 ∧
+         LIST_REL
+            (λ(x1,x2,x3) (y1,y2,y3).
+                 x1 = y1 ∧ x2 = y2 ∧ lift_rel x3 y3) ys1 ys2 ∧
+         LIST_REL
+            (λ(x1,x2,x3) (y1,y2,y3). x1 = y1 ∧ x2 = y2 ∧ d2b_rel x3 y3) ys2 ys’ by
+   (qpat_x_assum ‘LIST_REL _ xs ys’ mp_tac
+    \\ qpat_x_assum ‘EVERY _ (MAP _ xs)’ mp_tac
+    \\ qid_spec_tac ‘ys’ \\ qid_spec_tac ‘xs’
+    \\ rpt $ pop_assum kall_tac
+    \\ Induct \\ fs [PULL_EXISTS,UNCURRY,PULL_FORALL,EXISTS_PROD]
+    \\ rw [] \\ last_x_assum drule_all \\ rw []
+    \\ rpt $ first_assum $ irule_at Any
+    \\ imp_res_tac to_thunk_freevars \\ fs [])
+  \\ pop_assum $ irule_at Any
+  \\ pop_assum $ irule_at Any
+  \\ pop_assum $ irule_at Any
+  \\ pop_assum $ irule_at Any
+  \\ imp_res_tac to_thunk_freevars \\ fs []
+  \\ Cases_on ‘eopt’ \\ gvs [OPTREL_SIMP,PULL_EXISTS]
+  \\ rpt $ first_assum $ irule_at Any
+  \\ imp_res_tac to_thunk_freevars \\ fs []
 QED
 
 (*
